theories/Alpha/RenameApart_Alpha.v
@@ -1,0 +1,93 @@
+Require Import CSet Util Map.
+Require Import Env IL Alpha Fresh Annotation RenamedApart SetOperations.
+Require Import LabelsDefined PairwiseDisjoint RenameApart.
+
+Set Implicit Arguments.
+
+Lemma rename_apart_alpha' G ϱ ϱ' s
+  : lookup_set ϱ (freeVars s) ⊆ G
+  -> inverse_on (freeVars s) ϱ ϱ'
+  -> alpha ϱ' ϱ (snd (renameApart' ϱ G s)) s.
+Proof.
+  revert G ϱ ϱ'.
+  sind s; destruct s; simpl; intros; repeat let_pair_case_eq; subst;
+  simpl in * |- *; eauto using alpha.
+
+  - econstructor. eapply alpha_exp_sym. eapply alpha_exp_rename_injective.
+    eapply inverse_on_incl; try eassumption. eauto with cset.
+    eapply IH; eauto.
+    + rewrite <- H at 3. rewrite lookup_set_update_in_union; eauto.
+      cset_tac; intuition. right.
+      eapply lookup_set_union_incl; eauto. lset_tac.
+    + eapply inverse_on_update_inverse. intuition.
+      eapply inverse_on_incl; try eassumption. cset_tac; eauto.
+      assert (lookup_set ϱ (freeVars s \ {{x}}) ⊆
+                         lookup_set ϱ ((freeVars s \ {{x}}) ∪ Exp.freeVars e)).
+      rewrite lookup_set_union; cset_tac; intuition.
+      rewrite H1, H. eapply fresh_spec; eauto.
+  - econstructor; eauto.
+    + eapply alpha_op_sym. eapply alpha_op_rename_injective.
+      eapply inverse_on_incl; try eassumption. eapply incl_right.
+    + eapply IH; eauto.
+      * eapply Subset_trans; try eassumption. eapply lookup_set_incl; [intuition|].
+        rewrite union_assoc, union_comm. eapply incl_right.
+      * eapply inverse_on_incl; try eassumption.
+        rewrite union_assoc, union_comm. eapply incl_right.
+    + eapply IH; eauto.
+      * rewrite <- H at 1. repeat rewrite lookup_set_union; cset_tac; intuition.
+      * eapply inverse_on_incl; try eassumption.
+        cset_tac; intuition.
+  - econstructor. rewrite map_length; eauto.
+    intros. edestruct map_get_4; eauto; dcr; get_functional; subst.
+    eapply alpha_op_sym. eapply alpha_op_rename_injective.
+    eapply inverse_on_incl; try eassumption. eapply incl_list_union; try reflexivity.
+    eapply map_get_1; eauto.
+
+  - econstructor; eauto. eapply alpha_op_sym.
+    eapply alpha_op_rename_injective.
+    eapply inverse_on_incl; try eassumption. reflexivity.
+  - econstructor.
+    + rewrite rev_length, renameApartF_length; eauto.
+    + intros. eapply get_rev in H1.
+      rewrite renameApartF_length in H1.
+      edestruct get_fst_renameApartF as [? [? [? ]]]; dcr; eauto.
+      exploit (get_range H2).
+      orewrite (length F - S (length F - S n) = n) in H4. get_functional; subst.
+      eauto.
+    + intros.
+      eapply get_rev in H1.
+      rewrite renameApartF_length in H1.
+      edestruct get_fst_renameApartF as [? [? [? ]]]; dcr; eauto.
+      exploit (get_range H2).
+      orewrite (length F - S (length F - S n) = n) in H4. get_functional; subst.
+      rewrite H6.
+      erewrite renameApart'_agree. eapply IH; eauto.
+      * rewrite lookup_set_update_with_list_in_union_length; eauto.
+        eapply union_subset_3; eauto.
+        rewrite <- H5.
+        rewrite <- H.
+        eapply lookup_set_incl; eauto.
+        eapply incl_union_left.
+        eapply incl_list_union. eapply map_get_1; eauto. reflexivity.
+      * eapply inverse_on_update_fresh; eauto.
+        eapply inverse_on_incl; try eassumption. eauto.
+        eapply incl_union_left.
+        eapply incl_list_union. eapply map_get_1; eauto. reflexivity.
+        symmetry. eapply disj_1_incl; eauto.
+        rewrite <- H. eapply lookup_set_incl; eauto.
+        eapply incl_union_left.
+        eapply incl_list_union. eapply map_get_1; eauto. reflexivity.
+      * symmetry. eapply agree_on_incl; eauto with cset.
+    + eapply IH; eauto.
+      * rewrite <- H at 1.
+        rewrite lookup_set_union; eauto with cset.
+      * eapply inverse_on_incl; try eassumption. eauto.
+Qed.
+
+Lemma rename_apart_alpha s
+  : alpha id id (rename_apart s) s.
+Proof.
+  eapply rename_apart_alpha'.
+  + eapply lookup_set_on_id; reflexivity.
+  + eapply inverse_on_id.
+Qed.
