theories/Compiler.v
@@ -150,12 +150,11 @@ Print all.
 
 Definition fromILF (s:stmt) : status stmt :=
   let s_eae := EAE.compile s in
-  let (s_dcve, lv) := DCVE Liveness.Functional s_eae in
-  let s_ra := rename_apart s_dcve in
-  let (_, nlv) := RenameApart_Liveness.renameApart_live id (freeVars s_dcve) s_dcve lv in
-  let fvl := to_list (getAnn nlv) in
+  let s_ra := rename_apart s_eae in
+  let (s_dcve, lv) := DCVE Liveness.Functional s_ra in
+  let fvl := to_list (getAnn lv) in
   let ϱ := CMap.update_map_with_list fvl fvl (@MapInterface.empty var _ _ _) in
-  sdo ϱ' <- AllocationAlgo.regAssign s_ra nlv ϱ;
+  sdo ϱ' <- AllocationAlgo.regAssign s_ra lv ϱ;
     let s_allocated := rename (CMap.findt ϱ' 0) s_ra in
     let s_lowered := ParallelMove.lower parallel_move
                                        nil
