theories/Infra/PE.v
@@ -1,0 +1,78 @@
+Require Import CSet.
+
+Set Implicit Arguments.
+
+Instance prod_eq_refl X Y R R' `{Reflexive X R} `{Reflexive Y R'}
+  : Reflexive (prod_eq R R').
+Proof.
+  hnf; intros. destruct x; econstructor; reflexivity.
+Qed.
+
+Instance pe_sym X Y R R' `{Symmetric X R} `{Symmetric Y R'}
+  : Symmetric (prod_eq R R').
+Proof.
+  hnf; intros. inv H1; econstructor; eauto.
+Qed.
+
+Instance pe_trans  X Y R R' `{Transitive X R} `{Transitive Y R'}
+  : Transitive (prod_eq R R').
+Proof.
+  hnf; intros ? ? ? B C.
+  invc B; invc C; econstructor; eauto.
+Qed.
+
+Instance pe_morphism X Y (R:relation X) `{Transitive _ R}
+         (R':relation Y) `{Transitive _ R'}
+ : Proper ((flip (prod_eq R R')) ==> prod_eq R R' ==> impl) (prod_eq R R').
+Proof.
+  unfold Proper, respectful.
+  intros. inv H1; inv H2; inversion 1; subst; econstructor; eauto.
+Qed.
+
+Instance pe_morphism' X `{OrderedType X}
+ : Proper (prod_eq Equal Equal ==> prod_eq Equal Equal ==> iff) (prod_eq Equal Subset).
+Proof.
+  unfold Proper, respectful.
+  intros. inv H0; inv H1; split; inversion 1; subst; econstructor; eauto;
+  cset_tac; firstorder.
+Qed.
+
+Instance pe_morphism'' X `{OrderedType X}
+ : Proper (prod_eq Equal Equal ==> prod_eq Equal Equal ==> impl) (prod_eq Equal Subset).
+Proof.
+  unfold Proper, respectful.
+  intros. inv H0; inv H1; inversion 1; subst; econstructor; eauto;
+  cset_tac; firstorder.
+Qed.
+
+Instance pe_morphism''' X `{OrderedType X}
+ : Proper (prod_eq Equal Equal ==> prod_eq Equal Equal ==> flip impl) (prod_eq Equal Subset).
+Proof.
+  unfold Proper, respectful.
+  intros. inv H0; inv H1; inversion 1; subst; econstructor; eauto;
+  cset_tac; firstorder.
+Qed.
+
+
+Lemma prod_eq_proj1 X Y R R' (p p':X*Y)
+  : prod_eq R R' p p'
+    -> R (fst p) (fst p').
+Proof.
+  inversion 1; eauto.
+Qed.
+
+Lemma prod_eq_proj2 X Y R R' (p p':X*Y)
+  : prod_eq R R' p p'
+    -> R' (snd p) (snd p').
+Proof.
+  inversion 1; eauto.
+Qed.
+
+Hint Resolve prod_eq_intro.
+
+Lemma pe_eta_split X Y R R' (x:X* Y) y z
+  : prod_eq R R' (fst x, snd x) (y, z)
+    -> prod_eq R R' x (y,z).
+Proof.
+  destruct x; eauto.
+Qed.
